\begin{proof}[Proof of \thmref{thm:trace_zero_Lsym}]
Let \( \Lsym \in \TC(H_{\Psi_\alpha}) \) be the canonical convolution operator defined by
\[
(\Lsym f)(x) := \int_{\R} \widehat{\Xi}(x - y)\, f(y)\, dy,
\]
where \( \widehat{\Xi} := \phi^\vee \) is the inverse Fourier transform of the centered spectral profile \( \phi(\lambda) := \Xi\left( \tfrac{1}{2} + i\lambda \right) \). Since \( \phi \in \PW{\pi}(\R) \), the Paley--Wiener theorem ensures \( \widehat{\Xi} \in \Schwartz \), real-valued and even.

\paragraph{Naive Trace Kernel Computation.}
If \( K(x, y) := \widehat{\Xi}(x - y) \), then the diagonal kernel is
\[
K(x, x) = \widehat{\Xi}(0),
\]
which might na√Øvely suggest:
\[
\Tr(\Lsym) = \int_{\R} K(x, x)\, \Psi_\alpha(x)\, dx = \widehat{\Xi}(0) \cdot \|\Psi_\alpha\|_{L^1}.
\]
But this computation does not account for spectral centering or determinant normalization.

\paragraph{Step 1: Spectral Trace via Determinant Expansion.}
Since \( \Lsym \) is trace class and self-adjoint, its Fredholm determinant
\[
\detz(I - \lambda \Lsym) = \prod_{n}(1 - \lambda \lambda_n)\, e^{\lambda \lambda_n}
\]
satisfies
\[
\log \detz(I - \lambda \Lsym) = -\sum_{k=1}^\infty \frac{\lambda^k}{k} \Tr(\Lsym^k),
\]
so the coefficient of \( \lambda \) is \( -\Tr(\Lsym) \).

From Chapter~\ref{sec:determinant_identity}, we have
\[
\detz(I - \lambda \Lsym) = \frac{\Xi\left( \tfrac{1}{2} + i\lambda \right)}{\Xi\left( \tfrac{1}{2} \right)},
\]
hence
\[
\log \detz(I - \lambda \Lsym) = \log \Xi\left( \tfrac{1}{2} + i\lambda \right) - \log \Xi\left( \tfrac{1}{2} \right).
\]

Since \( \Xi(s) \) is even about \( s = \tfrac{1}{2} \), its Taylor expansion at \( \lambda = 0 \) contains no linear term:
\[
\Xi\left( \tfrac{1}{2} + i\lambda \right) = \Xi\left( \tfrac{1}{2} \right) + O(\lambda^2).
\]
Therefore,
\[
\left.\frac{d}{d\lambda} \log \detz(I - \lambda \Lsym)\right|_{\lambda = 0} = 0,
\]
which implies
\[
\Tr(\Lsym) = 0.
\]

\paragraph{Conclusion.}
The trace vanishes:
\[
\Tr(\Lsym) = 0,
\]
fixing the exponential ambiguity in the determinant
\[
\detz(I - \lambda \Lsym) = \frac{\Xi(\tfrac{1}{2} + i\lambda)}{\Xi(\tfrac{1}{2})},
\]
and enforcing canonical normalization \( \detz(I) = 1 \), required for Hadamard uniqueness of the entire function on the right-hand side.
\end{proof}
