\begin{proof}[Proof of \lemref{lem:spectral_zero_encoding}]
From the determinant identity (see \cref{sec:determinant_identity}), we have:
\[
\det\nolimits_\zeta(I - \lambda L_{\sym}) = \frac{\XiR\left( \tfrac{1}{2} + i\lambda \right)}{\XiR\left( \tfrac{1}{2} \right)},
\]
where \( \XiR(s) \) is the completed Riemann zeta function. The zeros of the determinant coincide with the zeros of \( \XiR(\tfrac{1}{2} + i\lambda) \), and their multiplicities are preserved via Hadamard factorization.

\paragraph{Forward Map.}
Let \( \rho \in \C \) be a nontrivial zero of \( \zetaR(s) \), so \( \XiR(\rho) = 0 \) and \( \rho = \tfrac{1}{2} + i\lambda \) for some \( \lambda \in \C \). Define
\[
\mu_\rho := \frac{1}{i(\rho - \tfrac{1}{2})} = \frac{1}{\lambda}.
\]
Then the determinant vanishes at \( \lambda \), so by analytic Fredholm theory,
\[
\mu_\rho = \lambda^{-1} \in \Spec(L_{\sym}) \setminus \{0\}.
\]
The multiplicity of the zero \( \rho \) of \( \XiR(s) \) equals the algebraic multiplicity of the eigenvalue \( \mu_\rho \), since both are encoded in the same Hadamard product.

\paragraph{Reverse Map.}
Conversely, let \( \mu \in \Spec(L_{\sym}) \setminus \{0\} \). Then the determinant vanishes at \( \lambda := \mu^{-1} \), so
\[
\XiR\left(\tfrac{1}{2} + i\lambda\right) = 0.
\]
Set
\[
\rho := \tfrac{1}{2} + i\lambda = \tfrac{1}{2} + i \mu^{-1}.
\]
Then \( \zetaR(\rho) = 0 \), and \( \mu = \mu_\rho \). The multiplicity of \( \mu \) as an eigenvalue equals the order of vanishing of \( \XiR \) at \( \rho \), completing the bijection.

\paragraph{Conclusion.}
The map
\[
\rho \mapsto \mu_\rho := \frac{1}{i}(\rho - \tfrac{1}{2})
\]
defines a multiplicity-preserving bijection between the nontrivial zeros of \( \zetaR(s) \) and the nonzero spectrum of \( L_{\sym} \), as claimed.
\end{proof}
