\begin{proof}[Proof of \lemref{lem:fredholm_zero_spectral_map}]
Let
\[
f(\lambda) := \det\nolimits_\zeta(I - \lambda L_{\sym}) = \frac{\XiR(\tfrac{1}{2} + i\lambda)}{\XiR(\tfrac{1}{2})},
\]
as given by \thmref{thm:det_identity_revised}.

\paragraph{(i) Forward Map.}
Let \( \rho = \tfrac{1}{2} + i\gamma \) be a nontrivial zero of \( \zetaR(s) \), with multiplicity \( m_\rho \). Then \( f(\lambda) \) vanishes at
\[
\lambda_\rho := i(\rho - \tfrac{1}{2}) = \gamma
\]
with order \( m_\rho \), since \( \XiR(\tfrac{1}{2} + i\lambda) \) inherits all zeros from \( \zetaR(s) \). By the Hadamard product structure of the determinant, we have:
\[
f(\lambda) = \prod_{\mu \in \Spec(L_{\sym})} (1 - \lambda \mu)^{\operatorname{mult}(\mu)},
\]
so that \( \lambda_\rho = 1/\mu_\rho \) is a zero of order \( m_\rho \). Hence,
\[
\mu_\rho := \frac{1}{\lambda_\rho} = \frac{1}{i(\rho - \tfrac{1}{2})} \in \Spec(L_{\sym})
\]
is an eigenvalue with multiplicity equal to the order of vanishing of \( \zetaR(s) \) at \( \rho \).

\paragraph{(ii) Inverse Map.}
Let \( \mu \in \Spec(L_{\sym}) \setminus \{0\} \), with multiplicity \( m \). Then \( \lambda := \mu^{-1} \) is a zero of \( f(\lambda) \) of order \( m \), and corresponds to a unique value
\[
\rho := \tfrac{1}{2} + \frac{1}{i\mu}
\]
such that \( \zetaR(\rho) = 0 \), and
\[
\mu = \mu_\rho := \frac{1}{i(\rho - \tfrac{1}{2})}.
\]

\paragraph{(iii) Bijection of Multisets.}
The map \( \rho \mapsto \mu_\rho \) is injective, since \( \rho \mapsto \lambda_\rho := i(\rho - \tfrac{1}{2}) \) is injective. By parts (i)â€“(ii), this map is also surjective and multiplicity-preserving. Hence, the zero set of \( f(\lambda) \) is precisely
\[
\left\{ \lambda_\rho := i(\rho - \tfrac{1}{2}) : \zetaR(\rho) = 0 \right\},
\]
and the inverse map \( \mu \mapsto \rho = \tfrac{1}{2} + \frac{1}{i\mu} \) recovers the corresponding zeta zero. The canonical map \( \rho \mapsto \mu_\rho \) thus defines a bijection of multisets between the nontrivial zeros of \( \zetaR(s) \) and the nonzero spectrum of \( L_{\sym} \).
\end{proof}
