\begin{proof}[Proof of Lemma~\ref{lem:no_extraneous_zeros}]
The canonical determinant is given by
\[
f(\lambda) := \det\nolimits_\zeta(I - \lambda L_{\mathrm{sym}})
= \frac{\Xi\left(\tfrac{1}{2} + i\lambda\right)}{\Xi\left(\tfrac{1}{2}\right)}.
\]
As \( \Xi(s) \) is entire of order 1 and genus 1, its Hadamard factorization takes the form:
\[
\Xi\left(\tfrac{1}{2} + i\lambda\right)
= \Xi\left(\tfrac{1}{2}\right)
\prod_{\rho} \left(1 - \frac{\lambda}{\mu_\rho} \right)
\exp\left( \frac{\lambda}{\mu_\rho} \right),
\]
where \( \mu_\rho := 1/i(\rho - \tfrac{1}{2}) \), and the product is taken over all nontrivial zeros \( \rho \) of \( \zeta(s) \).

The logarithmic derivative of \( f \) is:
\[
\frac{f'(\lambda)}{f(\lambda)}
= \sum_\rho \left( \frac{1}{\lambda - \mu_\rho} + \frac{1}{\mu_\rho} \right).
\]
This expression reveals that all poles of \( f'/f \) lie precisely at \( \lambda = \mu_\rho \), with multiplicity matching the order of vanishing of \( \zeta \) at \( \rho \).

Now, if the Hadamard exponential prefactor
\[
\exp\left( \sum_\rho \frac{\lambda}{\mu_\rho} \right)
\]
were to introduce new zeros, then \( f(\lambda) \) would vanish at points \( \lambda \notin \{ \mu_\rho \} \), contradicting the spectral correspondence established in Chapter~\ref{sec:spectral_correspondence} and violating the trace-zero normalization \( f(0) = 1 \).

Since
\[
\operatorname{Tr}(L_{\mathrm{sym}}) = \sum_n \mu_n = 0,
\]
the exponential term introduces no poles or zeros: it is entire and non-vanishing. Therefore, all zeros of \( f \) come from the product over \( \mu_\rho \).

\end{proof}
% 